src/Init/Data/String/Pattern/Char.lean
@@ -32,31 +32,17 @@ def iter (c : Char) (s : Slice) : Std.Iter (α := ForwardCharSearcher c s) (Sear
   { internalState := { currPos := s.startPos }}
 
 instance (s : Slice) : Std.Iterators.Iterator (ForwardCharSearcher c s) Id (SearchStep s) where
-  IsPlausibleStep it
-    | .yield it' out =>
-      ∃ h1 : it.internalState.currPos ≠ s.endPos,
-        it'.internalState.currPos = it.internalState.currPos.next h1 ∧
-        match out with
-        | .matched startPos endPos =>
-          it.internalState.currPos = startPos ∧
-          it'.internalState.currPos = endPos ∧
-          it.internalState.currPos.get h1 = c
-        | .rejected startPos endPos =>
-          it.internalState.currPos = startPos ∧
-          it'.internalState.currPos = endPos ∧
-          it.internalState.currPos.get h1 ≠ c
-    | .skip _ => False
-    | .done => it.internalState.currPos = s.endPos
-  step := fun ⟨⟨currPos⟩⟩ =>
-    if h1 : currPos = s.endPos then
-      pure (.deflate ⟨.done, by simp [h1]⟩)
-    else
-      let nextPos := currPos.next h1
-      let nextIt := ⟨⟨nextPos⟩⟩
-      if h2 : currPos.get h1 = c then
-        pure (.deflate ⟨.yield nextIt (.matched currPos nextPos), by simp [h1, h2, nextIt, nextPos]⟩)
+  step
+    | ⟨⟨currPos⟩⟩ => do
+      if h1 : currPos = s.endPos then
+        return .done
       else
-        pure (.deflate ⟨.yield nextIt (.rejected currPos nextPos), by simp [h1, h2, nextIt, nextPos]⟩)
+        let nextPos := currPos.next h1
+        let nextIt := ⟨⟨nextPos⟩⟩
+        if currPos.get h1 = c then
+          return .yield nextIt (.matched currPos nextPos)
+        else
+          return .yield nextIt (.rejected currPos nextPos)
 
 def finitenessRelation : Std.Iterators.FinitenessRelation (ForwardCharSearcher s c) Id where
   rel := InvImage WellFoundedRelation.rel (fun it => it.internalState.currPos)
@@ -64,12 +50,12 @@ def finitenessRelation : Std.Iterators.FinitenessRelation (ForwardCharSearcher s
   subrelation {it it'} h := by
     simp_wf
     obtain ⟨step, h, h'⟩ := h
-    cases step
-    · cases h
-      obtain ⟨_, h2, _⟩ := h'
-      simp [h2]
+    simp only [Std.Iterators.IterM.IsPlausibleStep, MonadAttach.CanReturn,
+      Std.Iterators.Iterator.step] at h'
+    split at h'
     · cases h'
-    · cases h
+      cases h
+    · split at h' <;> (cases h'; cases h; simp)
 
 instance : Std.Iterators.Finite (ForwardCharSearcher s c) Id :=
   .of_finitenessRelation finitenessRelation
@@ -96,32 +82,17 @@ def iter (c : Char) (s : Slice) : Std.Iter (α := BackwardCharSearcher s) (Searc
   { internalState := { currPos := s.endPos, needle := c }}
 
 instance (s : Slice) : Std.Iterators.Iterator (BackwardCharSearcher s) Id (SearchStep s) where
-  IsPlausibleStep it
-    | .yield it' out =>
-      it.internalState.needle = it'.internalState.needle ∧
-      ∃ h1 : it.internalState.currPos ≠ s.startPos,
-        it'.internalState.currPos = it.internalState.currPos.prev h1 ∧
-        match out with
-        | .matched startPos endPos =>
-          it.internalState.currPos = endPos ∧
-          it'.internalState.currPos = startPos ∧
-          (it.internalState.currPos.prev h1).get Pos.prev_ne_endPos = it.internalState.needle
-        | .rejected startPos endPos =>
-          it.internalState.currPos = endPos ∧
-          it'.internalState.currPos = startPos ∧
-          (it.internalState.currPos.prev h1).get Pos.prev_ne_endPos ≠ it.internalState.needle
-    | .skip _ => False
-    | .done => it.internalState.currPos = s.startPos
-  step := fun ⟨currPos, needle⟩ =>
-    if h1 : currPos = s.startPos then
-      pure (.deflate ⟨.done, by simp [h1]⟩)
-    else
-      let nextPos := currPos.prev h1
-      let nextIt := ⟨nextPos, needle⟩
-      if h2 : nextPos.get Pos.prev_ne_endPos = needle then
-        pure (.deflate ⟨.yield nextIt (.matched nextPos currPos), by simp [h1, h2, nextIt, nextPos]⟩)
+  step
+    | ⟨currPos, needle⟩ => do
+      if h1 : currPos = s.startPos then
+        return .done
       else
-        pure (.deflate ⟨.yield nextIt (.rejected nextPos currPos), by simp [h1, h2, nextIt, nextPos]⟩)
+        let nextPos := currPos.prev h1
+        let nextIt := ⟨nextPos, needle⟩
+        if nextPos.get Pos.prev_ne_endPos = needle then
+          return .yield nextIt (.matched nextPos currPos)
+        else
+          return .yield nextIt (.rejected nextPos currPos)
 
 def finitenessRelation : Std.Iterators.FinitenessRelation (BackwardCharSearcher s) Id where
   rel := InvImage WellFoundedRelation.rel (fun it => it.internalState.currPos.down)
@@ -129,12 +100,13 @@ def finitenessRelation : Std.Iterators.FinitenessRelation (BackwardCharSearcher 
   subrelation {it it'} h := by
     simp_wf
     obtain ⟨step, h, h'⟩ := h
-    cases step
-    · cases h
-      obtain ⟨_, h1, h2, _⟩ := h'
-      simp [h2]
+    simp only [Std.Iterators.IterM.IsPlausibleStep, MonadAttach.CanReturn,
+      Std.Iterators.Iterator.step] at h'
+    split at h'
     · cases h'
-    · cases h
+      cases h
+    · split at h' <;> (cases h'; cases h; simp)
+    simp_wf
 
 instance : Std.Iterators.Finite (BackwardCharSearcher s) Id :=
   .of_finitenessRelation finitenessRelation
