src/Std/Data/Iterators/Combinators/Monadic/DropWhile.lean
@@ -11,6 +11,7 @@ public import Init.Data.Iterators.Consumers.Monadic.Collect
 public import Init.Data.Iterators.Consumers.Monadic.Loop
 public import Init.Data.Iterators.Internal.Termination
 public import Init.Data.Iterators.PostconditionMonad
+import Init.Control.Lawful.MonadAttach.Lemmas
 
 @[expose] public section
 
@@ -40,26 +41,11 @@ Internal state of the `dropWhile` combinator. Do not depend on its internals.
 -/
 @[unbox]
 structure DropWhile (α : Type w) (m : Type w → Type w') (β : Type w)
-    (P : β → PostconditionT m (ULift Bool)) where
+    (P : β → m (ULift Bool)) where
   /-- Internal implementation detail of the iterator library. -/
   dropping : Bool
   /-- Internal implementation detail of the iterator library. -/
   inner : IterM (α := α) m β
-
-/--
-Constructs intermediate states of an iterator created with the combinator
-`IterM.dropWhileWithPostcondition`.
-When `it.dropWhileWithPostcondition P` has stopped dropping elements, its new state cannot be
-created directly with `IterM.dropWhileWithPostcondition` but only with
-`Intermediate.dropWhileWithPostcondition`.
-
-`Intermediate.dropWhileWithPostcondition` is meant to be used only for internally or for
-verification purposes.
--/
-@[always_inline, inline]
-def IterM.Intermediate.dropWhileWithPostcondition (P : β → PostconditionT m (ULift Bool))
-    (dropping : Bool) (it : IterM (α := α) m β) :=
-  (toIterM (DropWhile.mk (P := P) dropping it) m β : IterM m β)
 
 /--
 Constructs intermediate states of an iterator created with the combinator `IterM.dropWhileM`.
@@ -70,8 +56,8 @@ directly with `IterM.dropWhileM` but only with `Intermediate.dropWhileM`.
 -/
 @[always_inline, inline]
 def IterM.Intermediate.dropWhileM [Monad m] (P : β → m (ULift Bool)) (dropping : Bool)
-    (it : IterM (α := α) m β) :=
-  (IterM.Intermediate.dropWhileWithPostcondition (PostconditionT.lift ∘ P) dropping it : IterM m β)
+    (it : IterM (α := α) m β) : IterM (α := DropWhile α m β P) m β :=
+  toIterM ⟨dropping, it⟩ m β
 
 /--
 Constructs intermediate states of an iterator created with the combinator `IterM.dropWhile`.
@@ -84,48 +70,6 @@ directly with `IterM.dropWhile` but only with `Intermediate.dropWhile`.
 def IterM.Intermediate.dropWhile [Monad m] (P : β → Bool) (dropping : Bool)
     (it : IterM (α := α) m β) :=
   (IterM.Intermediate.dropWhileM (pure ∘ ULift.up ∘ P) dropping it : IterM m β)
-
-/--
-*Note: This is a very general combinator that requires an advanced understanding of monads,
-dependent types and termination proofs. The variants `dropWhile` and `dropWhileM` are easier to use
-and sufficient for most use cases.*
-
-Given an iterator `it` and a monadic predicate `P`, `it.dropWhileWithPostcondition P` is an iterator
-that emits the values emitted by `it` starting from the first value that is rejected by `P`.
-The elements before are dropped.
-
-`P` is expected to return `PostconditionT m (ULift Bool)`. The `PostconditionT` transformer allows
-the caller to intrinsically prove properties about `P`'s return value in the monad `m`, enabling
-termination proofs depending on the specific behavior of `P`.
-
-**Marble diagram (ignoring monadic effects):**
-
-Assuming that the predicate `P` accepts `a` and `b` but rejects `c`:
-
-```text
-it                                ---a----b---c--d-e--⊥
-it.dropWhileWithPostcondition P   ------------c--d-e--⊥
-
-it                                ---a----⊥
-it.dropWhileWithPostcondition P   --------⊥
-```
-
-**Termination properties:**
-
-* `Finite` instance: only if `it` is finite
-* `Productive` instance: only if `it` is finite
-
-Depending on `P`, it is possible that `it.dropWhileWithPostcondition P` is finite (or productive) although
-`it` is not. In this case, the `Finite` (or `Productive`) instance needs to be proved manually.
-
-**Performance:**
-
-This combinator calls `P` on each output of `it` until the predicate evaluates to false. After
-that, the combinator incurs an additional O(1) cost for each value emitted by `it`.
--/
-@[always_inline, inline]
-def IterM.dropWhileWithPostcondition (P : β → PostconditionT m (ULift Bool)) (it : IterM (α := α) m β) :=
-  (Intermediate.dropWhileWithPostcondition P true it : IterM m β)
 
 /--
 Given an iterator `it` and a monadic predicate `P`, `it.dropWhileM P` is an iterator that
@@ -198,51 +142,25 @@ that, the combinator incurs an addictional O(1) cost for each value emitted by `
 -/
 @[always_inline, inline]
 def IterM.dropWhile [Monad m] (P : β → Bool) (it : IterM (α := α) m β) :=
-  (Intermediate.dropWhile P true it: IterM m β)
-
-/--
-`it.PlausibleStep step` is the proposition that `step` is a possible next step from the
-`dropWhile` iterator `it`. This is mostly internally relevant, except if one needs to manually
-prove termination (`Finite` or `Productive` instances, for example) of a `dropWhile` iterator.
--/
-inductive DropWhile.PlausibleStep [Iterator α m β] {P} (it : IterM (α := DropWhile α m β P) m β) :
-    (step : IterStep (IterM (α := DropWhile α m β P) m β) β) → Prop where
-  | yield : ∀ {it' out}, it.internalState.inner.IsPlausibleStep (.yield it' out) →
-      it.internalState.dropping = false →
-      PlausibleStep it (.yield (IterM.Intermediate.dropWhileWithPostcondition P false it') out)
-  | skip : ∀ {it'}, it.internalState.inner.IsPlausibleStep (.skip it') →
-      PlausibleStep it (.skip (IterM.Intermediate.dropWhileWithPostcondition P it.internalState.dropping it'))
-  | done : it.internalState.inner.IsPlausibleStep .done → PlausibleStep it .done
-  | start : ∀ {it' out}, it.internalState.inner.IsPlausibleStep (.yield it' out) →
-      it.internalState.dropping = true → (P out).Property (.up false) →
-      PlausibleStep it (.yield (IterM.Intermediate.dropWhileWithPostcondition P false it') out)
-  | dropped : ∀ {it' out}, it.internalState.inner.IsPlausibleStep (.yield it' out) →
-      it.internalState.dropping = true → (P out).Property (.up true) →
-      PlausibleStep it (.skip (IterM.Intermediate.dropWhileWithPostcondition P true it'))
+  (Intermediate.dropWhile P true it : IterM m β)
 
 @[always_inline, inline]
 instance DropWhile.instIterator [Monad m] [Iterator α m β] {P} :
     Iterator (DropWhile α m β P) m β where
-  IsPlausibleStep := DropWhile.PlausibleStep
   step it := do
-    match (← it.internalState.inner.step).inflate with
-    | .yield it' out h =>
-      if h' : it.internalState.dropping = true then
-        match ← (P out).operation with
-        | ⟨.up true, h''⟩ =>
-          return .deflate <| .skip (IterM.Intermediate.dropWhileWithPostcondition P true it') (.dropped h h' h'')
-        | ⟨.up false, h''⟩ =>
-          return .deflate <| .yield (IterM.Intermediate.dropWhileWithPostcondition P false it') out (.start h h' h'')
-      else
-        return .deflate <| .yield (IterM.Intermediate.dropWhileWithPostcondition P false it') out
-            (.yield h (Bool.not_eq_true _ ▸ h'))
-    | .skip it' h =>
-      return .deflate <| .skip (IterM.Intermediate.dropWhileWithPostcondition P it.internalState.dropping it') (.skip h)
-    | .done h =>
-      return .deflate <| .done (.done h)
+    match ← it.internalState.inner.step with
+    | .yield it' out =>
+      if it.internalState.dropping = true then
+        match ← P out with
+        | .up true => return .skip (IterM.Intermediate.dropWhileM P true it')
+        | .up false => return .yield (IterM.Intermediate.dropWhileM P false it') out
+      else return .yield (IterM.Intermediate.dropWhileM P false it') out
+    | .skip it' => return .skip (IterM.Intermediate.dropWhileM P it.internalState.dropping it')
+    | .done => return .done
 
-private def DropWhile.instFinitenessRelation [Monad m] [Iterator α m β]
-    [Finite α m] {P} :
+private def DropWhile.instFinitenessRelation
+    [Monad m] [MonadAttach m] [LawfulMonad m] [LawfulMonadAttach m]
+    [Iterator α m β] [Finite α m] {P} :
     FinitenessRelation (DropWhile α m β P) m where
   rel := InvImage WellFoundedRelation.rel
       (IterM.finitelyManySteps ∘ DropWhile.inner ∘ IterM.internalState)
@@ -250,33 +168,39 @@ private def DropWhile.instFinitenessRelation [Monad m] [Iterator α m β]
     apply InvImage.wf
     exact WellFoundedRelation.wf
   subrelation {it it'} h := by
-    obtain ⟨step, h, h'⟩ := h
-    cases h'
-    case yield it' out k h' h'' =>
-      cases h
-      exact IterM.TerminationMeasures.Finite.rel_of_yield h'
-    case skip it' out h' =>
-      cases h
-      exact IterM.TerminationMeasures.Finite.rel_of_skip h'
-    case done _ =>
-      cases h
-    case start it' out h' h'' h''' =>
-      cases h
-      exact IterM.TerminationMeasures.Finite.rel_of_yield h'
-    case dropped it' out h' h'' h''' =>
-      cases h
-      exact IterM.TerminationMeasures.Finite.rel_of_yield h'
+    obtain ⟨step, hs, h'⟩ := h
+    obtain ⟨step', hs', h'⟩ := LawfulMonadAttach.canReturn_bind_imp' h'
+    cases step', hs' using PlausibleIterStep.casesOn'
+    · simp only at h'
+      split at h'
+      · obtain ⟨Px, hPx, h'⟩ := LawfulMonadAttach.canReturn_bind_imp' h'
+        split at h'
+        all_goals
+          cases LawfulMonadAttach.eq_of_canReturn_pure h'
+          cases hs
+          apply IterM.TerminationMeasures.Finite.rel_of_yield ‹_›
+      · cases LawfulMonadAttach.eq_of_canReturn_pure h'
+        cases hs
+        exact IterM.TerminationMeasures.Finite.rel_of_yield ‹_›
+    · cases LawfulMonadAttach.eq_of_canReturn_pure h'
+      cases hs
+      exact IterM.TerminationMeasures.Finite.rel_of_skip ‹_›
+    · cases LawfulMonadAttach.eq_of_canReturn_pure h'
+      cases hs
 
-instance DropWhile.instFinite [Monad m] [Iterator α m β] [Finite α m] {P} :
+instance DropWhile.instFinite
+    [Monad m] [MonadAttach m] [LawfulMonad m] [LawfulMonadAttach m]
+    [Iterator α m β] [Finite α m] {P} :
     Finite (DropWhile α m β P) m :=
   by exact Finite.of_finitenessRelation instFinitenessRelation
 
-instance DropWhile.instIteratorCollect [Monad m] [Monad n] [Iterator α m β] [Productive α m] {P} :
+instance DropWhile.instIteratorCollect [Monad m] [MonadAttach m] [Monad n]
+    [Iterator α m β] [Productive α m] {P} :
     IteratorCollect (DropWhile α m β P) m n :=
   .defaultImplementation
 
-instance DropWhile.instIteratorLoop [Monad m] [Monad n] [Iterator α m β] :
-    IteratorLoop (DropWhile α m β P) m n :=
+instance DropWhile.instIteratorLoop [Monad m] [MonadAttach m] [Monad n] [MonadAttach n]
+    [Iterator α m β] : IteratorLoop (DropWhile α m β P) m n :=
   .defaultImplementation
 
 end Std.Iterators
